examples/IsaTest.v
@@ -26,10 +26,12 @@ Local Ltac line i c := exact (ConstBit (rv32iToRaw c)).
 Local Ltac nop := exact (ConstBit (rv32iToRaw NOP)).
 Local Notation "'Program'" := (ConstT (Vector (Data rv32iLgDataBytes) rv32iAddrSize)).
 
+Definition branchTarget {sz} (ofs: nat) := natToWord sz (ofs * 4).
+
 (* Expected output : 2 *)
 Definition pgmJalTest1 : Program.
   init_pgm.
-  line 0 (JAL x0 (natToWord _ 5)).
+  line 0 (JAL x0 (branchTarget 5)).
   line 1 NOP.
   line 2 NOP.
   line 3 (LI x3 (natToWord _ 1)).
@@ -45,7 +47,7 @@ Defined.
 (* Expected output : 5 *)
 Definition pgmJalTest2 : Program.
   init_pgm.
-  line 0 (JAL x1 (natToWord _ 5)).
+  line 0 (JAL x1 (branchTarget 5)).
   line 1 NOP.
   line 2 NOP.
   line 3 NOP.
@@ -60,7 +62,7 @@ Defined.
 (* Expected output : 2 *)
 Definition pgmJalrTest1 : Program.
   init_pgm.
-  line 0 (LI x1 (natToWord _ 5)).
+  line 0 (LI x1 (branchTarget 5)).
   line 1 (JALR x1 x0 (natToWord _ 0)).
   line 2 NOP.
   line 3 NOP.
@@ -76,7 +78,7 @@ Defined.
 (* Expected output : 6 *)
 Definition pgmJalrTest2 : Program.
   init_pgm.
-  line 0 (LI x1 (natToWord _ 5)).
+  line 0 (LI x1 (branchTarget 5)).
   line 1 (JALR x1 x2 (natToWord _ 0)).
   line 2 NOP.
   line 3 NOP.
@@ -94,7 +96,7 @@ Definition pgmBeqTest : Program.
   init_pgm.
   line 0 (LI x1 (natToWord _ 5)).
   line 1 (LI x2 (natToWord _ 5)).
-  line 2 (BEQ x1 x2 (natToWord _ 3)).
+  line 2 (BEQ x1 x2 (branchTarget 3)).
   line 3 (LI x3 (natToWord _ 1)).
   line 4 (TOHOST x3).
   line 5 (LI x3 (natToWord _ 2)).
@@ -110,7 +112,7 @@ Definition pgmBneTest : Program.
   init_pgm.
   line 0 (LI x1 (natToWord _ 4)).
   line 1 (LI x2 (natToWord _ 5)).
-  line 2 (BNE x1 x2 (natToWord _ 3)).
+  line 2 (BNE x1 x2 (branchTarget 3)).
   line 3 (LI x3 (natToWord _ 1)).
   line 4 (TOHOST x3).
   line 5 (LI x3 (natToWord _ 2)).
@@ -126,7 +128,7 @@ Definition pgmBltTest : Program.
   init_pgm.
   line 0 (LI x1 (natToWord _ 4)).
   line 1 (LI x2 (natToWord _ 5)).
-  line 2 (BLT x1 x2 (natToWord _ 3)).
+  line 2 (BLT x1 x2 (branchTarget 3)).
   line 3 (LI x3 (natToWord _ 1)).
   line 4 (TOHOST x3).
   line 5 (LI x3 (natToWord _ 2)).
@@ -142,7 +144,7 @@ Definition pgmBgeTest : Program.
   init_pgm.
   line 0 (LI x1 (natToWord _ 5)).
   line 1 (LI x2 (natToWord _ 4)).
-  line 2 (BGE x1 x2 (natToWord _ 3)).
+  line 2 (BGE x1 x2 (branchTarget 3)).
   line 3 (LI x3 (natToWord _ 1)).
   line 4 (TOHOST x3).
   line 5 (LI x3 (natToWord _ 2)).
@@ -188,7 +190,7 @@ Definition pgmToHostTest (n: nat) : Program.
   line 0 (LI x3 (natToWord _ n)).
   line 1 (TOHOST x3).
   line 2 NOP.
-  line 3 (J (natToWord _ 30)). (* 3 + 30 == 1 *)
+  line 3 (J (branchTarget 30)). (* 3 + 30 == 1 *)
   nop. nop. nop. nop. nop. nop. nop. nop. 
   nop. nop. nop. nop. nop. nop. nop. nop. 
   nop. nop. nop. nop. nop. nop. nop. nop. 
@@ -201,7 +203,7 @@ Definition pgmSubTest: Program.
   line 0 (LI x1 (natToWord _ 5)).
   line 1 (LI x2 (natToWord _ 5)).
   line 2 (SUB x1 x2 x3).
-  line 3 (BEQ x3 x0 (natToWord _ 3)).
+  line 3 (BEQ x3 x0 (branchTarget 3)).
   line 4 (LI x4 (natToWord _ 1)).
   line 5 (TOHOST x4).
   line 6 (LI x4 (natToWord _ 2)).
@@ -218,7 +220,7 @@ Definition pgmSllTest: Program.
   line 1 (LI x2 (natToWord _ 2)).
   line 2 (SLL x1 x2 x3). (* x3 = x1 << x2 *)
   line 3 (LI x4 (natToWord _ 12)). (* 12 = 3 << 2 *)
-  line 4 (BEQ x3 x4 (natToWord _ 3)).
+  line 4 (BEQ x3 x4 (branchTarget 3)).
   line 5 (LI x5 (natToWord _ 1)).
   line 6 (TOHOST x5).
   line 7 (LI x5 (natToWord _ 2)).
@@ -235,7 +237,7 @@ Definition pgmSrlTest: Program.
   line 1 (LI x2 (natToWord _ 2)).
   line 2 (SRL x1 x2 x3). (* x3 = x1 >> x2 *)
   line 3 (LI x4 (natToWord _ 3)). (* 3 = 12 >> 2 *)
-  line 4 (BEQ x3 x4 (natToWord _ 3)).
+  line 4 (BEQ x3 x4 (branchTarget 3)).
   line 5 (LI x5 (natToWord _ 1)).
   line 6 (TOHOST x5).
   line 7 (LI x5 (natToWord _ 2)).
@@ -252,7 +254,7 @@ Definition pgmOrTest: Program.
   line 1 (LI x2 (natToWord _ 56)).
   line 2 (OR x1 x2 x3).
   line 3 (LI x4 (natToWord _ 63)).
-  line 4 (BEQ x3 x4 (natToWord _ 3)).
+  line 4 (BEQ x3 x4 (branchTarget 3)).
   line 5 (LI x5 (natToWord _ 1)).
   line 6 (TOHOST x5).
   line 7 (LI x5 (natToWord _ 2)).
@@ -268,7 +270,7 @@ Definition pgmAndTest: Program.
   line 0 (LI x1 (natToWord _ 7)).
   line 1 (LI x2 (natToWord _ 56)).
   line 2 (AND x1 x2 x3).
-  line 3 (BEQ x3 x0 (natToWord _ 3)).
+  line 3 (BEQ x3 x0 (branchTarget 3)).
   line 4 (LI x5 (natToWord _ 1)).
   line 5 (TOHOST x5).
   line 6 (LI x5 (natToWord _ 2)).
@@ -285,7 +287,7 @@ Definition pgmXorTest: Program.
   line 1 (LI x2 (natToWord _ 42)). (* 101010 *)
   line 2 (XOR x1 x2 x3).
   line 3 (LI x4 (natToWord _ 15)). (* 001111 *)
-  line 4 (BEQ x3 x4 (natToWord _ 3)).
+  line 4 (BEQ x3 x4 (branchTarget 3)).
   line 5 (LI x5 (natToWord _ 1)).
   line 6 (TOHOST x5).
   line 7 (LI x5 (natToWord _ 2)).
@@ -308,11 +310,11 @@ Definition pgmFibonacci (n: nat) : Program.
   line 7 (ADDI x9 x9 (natToWord _ 1)).
   line 8 (MV x8 x7).
   line 9 (MV x5 x8).
-  line 10 (BNE x6 x9 (natToWord _ 28)). (* 10 + 28 == 6 *)
+  line 10 (BNE x6 x9 (branchTarget 28)). (* 10 + 28 == 6 *)
   line 11 (TOHOST x5).
   line 12 (J (natToWord _ 3)). (* to 15 *)
   line 13 (LI x5 (natToWord _ 1)).
-  line 14 (J (natToWord _ 29)). (* 14 + 29 == 11 *)
+  line 14 (J (branchTarget 29)). (* 14 + 29 == 11 *)
   line 15 NOP.
   nop. nop. nop. nop. nop. nop. nop. nop. 
   nop. nop. nop. nop. nop. nop. nop. nop.
@@ -327,9 +329,9 @@ Definition pgmGcd (n m: nat) : Program.
   line 3 (SUB x9 x8 x5).
   line 4 (SUB x8 x9 x6).
   line 5 (MV x9 x7).
-  line 6 (BGE x8 x9 (natToWord _ 2)).
+  line 6 (BGE x8 x9 (branchTarget 2)).
   line 7 (MV x5 x7).
-  line 8 (BLT x4 x9 (natToWord _ 2)).
+  line 8 (BLT x4 x9 (branchTarget 2)).
   line 9 (MV x6 x4).
   line 10 (MV x4 x8).
   line 11 (MV x7 x9).
@@ -348,7 +350,7 @@ Definition pgmFactorial (n: nat) : Program.
   line 2 (LI x8 (natToWord _ (S n))).
   line 3 (MUL x4 x9 x4).
   line 4 (ADDI x9 x9 (natToWord _ 1)).
-  line 5 (BNE x9 x8 (natToWord _ 30)). (* 5 + 30 == 3 *)
+  line 5 (BNE x9 x8 (branchTarget 30)). (* 5 + 30 == 3 *)
   line 6 (TOHOST x4).
   nop. nop. nop. nop. nop. nop. nop. nop.
   nop. nop. nop. nop. nop. nop. nop. nop.
